theories/laws/utp_refine_laws.thy
@@ -30,6 +30,10 @@ lemma SeqR_disjunctive2:
   apply (utp_rel_auto_tac)
 done
 
+lemma RefineP_taut [simp]: 
+  "`p \<sqsubseteq> q` \<longleftrightarrow> p \<sqsubseteq> q"
+  by (simp add: less_eq_WF_PREDICATE_def)
+
 theorem RefineP_TrueP_refine [refine]:
   "true \<sqsubseteq> P"
   by (utp_pred_tac)
@@ -124,6 +128,19 @@ lemma SkipR_transport_refine [refine]:
   "\<lbrakk> D\<^sub>1 \<sharp> p; q \<sqsubseteq> p\<acute> \<rbrakk> \<Longrightarrow> q \<sqsubseteq> p \<and>\<^sub>p II"
   by (utp_rel_auto_tac)
 
+declare EvalP_SkipR [eval del]
+declare EvalP_SkipR_alt [eval]
+
+declare EvalP_SkipRA [eval del]
+declare EvalP_SkipRA_alt [eval]
+
+lemma SkipRA_refines_ImpliesP:
+  "\<lbrakk> vs1 \<subseteq> D\<^sub>0; - vs1 \<sharp> p; HOMOGENEOUS(vs2); vs1 \<subseteq> vs2 \<rbrakk> 
+   \<Longrightarrow> `p \<Rightarrow> p\<acute>` \<sqsubseteq> `II\<^bsub>vs2\<^esub>`"
+  apply (utp_pred_tac)
+  apply (metis EvalP_binding_equiv binding_equiv_subset in_vars_def le_inf_iff)
+done
+
 lemma AssignR_refinement [refine]:
   assumes
     "x \<in> UNDASHED" "v \<rhd>\<^sub>e x" "DASHED \<sharp> v" "q[v/\<^sub>px\<acute>] \<sqsubseteq> p"
@@ -151,13 +168,23 @@ qed
 
 lemma AssignRA_refinement [refine]:
   assumes
-    "HOMOGENEOUS xs" "xs \<subseteq> REL_VAR" "x \<in> xs" "x\<acute> \<in> xs" 
-    "v \<rhd>\<^sub>e x" "(VAR - in(xs)) \<sharp> v" "q[v/\<^sub>px\<acute>] \<sqsubseteq> p"
+    "HOMOGENEOUS xs" "xs \<subseteq> REL_VAR" "x \<in> in(xs)"
+    "v \<rhd>\<^sub>e x" "- in(xs) \<sharp> v" "q[v/\<^sub>px\<acute>] \<sqsubseteq> p"
   shows "(p \<Rightarrow>\<^sub>p q) \<sqsubseteq> x :=\<^bsub>xs\<^esub> v"
   using assms
-    apply (utp_pred_tac)
-    apply (safe)
-    apply (metis (lifting, no_types) DASHED_dash_not_DASHED UNDASHED_eq_dash_contra UnE binding_upd_triv in_member in_mono)
+  by (utp_pred_auto_tac, metis binding_upd_triv)
+
+lemma AssignRA_refinement_alt:
+  assumes "HOMOGENEOUS(xs)" "xs \<subseteq> REL_VAR" "x \<in> in(xs)"
+          "v \<rhd>\<^sub>e x" "- in(xs) \<sharp> p" "- in(xs) \<sharp> v"
+  shows "(p[v/\<^sub>px] \<Rightarrow>\<^sub>p p\<acute>) \<sqsubseteq> x :=\<^bsub>xs\<^esub> v"
+  using assms
+  apply (utp_pred_auto_tac)
+  apply (subst EvalP_binding_equiv[of _ _ _ "b(x :=\<^sub>b \<lbrakk>v\<rbrakk>\<^sub>eb)"])
+  apply (simp_all)
+  apply (subgoal_tac "x \<in> D\<^sub>0")
+  apply (simp add: binding_equiv_def urename)
+  apply (metis in_UNDASHED set_rev_mp)
 done
 
 end
