theories/tactics/utp_pred_tac.thy
@@ -352,3 +352,4 @@ lemma AndP_reorder_test :
   by (utp_pred_auto_tac)
 
 end
+
